generic/Zeta.AppSimulate.fst
@@ -8,6 +8,10 @@ let prefix_of_distinct_distinct
                   distinct_keys #adm sk'))
   = ()
 
+let of_key (#adm:_) (ki: app_key adm) (r: app_record adm)
+  = let k,_ = r in
+    k = ki
+
 let input_incorrect_idx (#adm:_) (st: app_state adm) (r: app_record adm)
   : bool
   = let k,v = r in
@@ -22,3 +26,14 @@ let input_correct (#adm: app_data_model)
                     st k = v)})
   = let open Zeta.SeqIdx in
     not (exists_elems_with_prop_comp (input_incorrect_idx st) inp)
+
+let refs_comp (#app:_) (fc: appfn_call app) (k: app_key app.adm)
+  : b:bool { b <==> refs fc k }
+  = let open Zeta.SeqIdx in
+    exists_elems_with_prop_comp (of_key k) fc.inp_c
+
+(* for a referenced key, return the parameter position index *)
+let refkey_idx (#app:_) (fc: appfn_call app) (k: app_key app.adm{fc `refs` k})
+  : i:_{let k',v = FStar.Seq.index fc.inp_c i in k' = k}
+  = let open Zeta.SeqIdx in
+    last_idx (of_key k) fc.inp_c
